@prefix adms: <http://www.w3.org/ns/adms#> .
@prefix cnt: <http://www.w3.org/2011/content#> .
@prefix dc: <http://purl.org/dc/elements/1.1/> .
@prefix dcat: <http://www.w3.org/ns/dcat#> .
@prefix dcatap: <http://data.europa.eu/r5r/> .
@prefix dct: <http://purl.org/dc/terms/> .
@prefix dctype: <http://purl.org/dc/dcmitype/> .
@prefix foaf: <http://xmlns.com/foaf/0.1/> .
@prefix geodcatap: <http://data.europa.eu/930/> .
@prefix gsp: <http://www.opengis.net/ont/geosparql#> .
@prefix locn: <http://www.w3.org/ns/locn#> .
@prefix odrl: <http://www.w3.org/ns/odrl/2/> .
@prefix org: <http://www.w3.org/ns/org#> .
@prefix owl: <http://www.w3.org/2002/07/owl#> .
@prefix prov: <http://www.w3.org/ns/prov#> .
@prefix rdf: <http://www.w3.org/1999/02/22-rdf-syntax-ns#> .
@prefix rdfs: <http://www.w3.org/2000/01/rdf-schema#> .
@prefix schema: <http://schema.org/> .
@prefix skos: <http://www.w3.org/2004/02/skos/core#> .
@prefix spdx: <http://spdx.org/rdf/terms#> .
@prefix time: <http://www.w3.org/2006/time#> .
@prefix vcard: <http://www.w3.org/2006/vcard/ns#> .
@prefix xml: <http://www.w3.org/XML/1998/namespace> .
@prefix xsd: <http://www.w3.org/2001/XMLSchema#> .

geodcatap:spatialResolutionAsScale a rdf:Property ;
  rdfs:label "spatial resolution as equivalent scale"@en ;
  rdfs:comment "Spatial resolution of a dataset expressed as equivalent scale, measured by using a representative fraction (e.g., 1:1,000, 1:1,000,000)."@en ;
  rdfs:range xsd:decimal .

geodcatap:spatialResolutionAsVerticalDistanceInMeters a rdf:Property ;
  rdfs:label "spatial resolution as equivalent scale"@en ;
  rdfs:comment "Spatial resolution of a dataset expressed as vertical distance, measured in metres."@en ;
  rdfs:range xsd:decimal .

geodcatap:spatialResolutionInDegrees a rdf:Property ;
  rdfs:label "spatial resolution as angular distance"@en ;
  rdfs:comment "Spatial resolution of a dataset expressed as angular distance, measured in decimal degrees."@en ;
  rdfs:range xsd:decimal .

